Add no_flush modality

src/high/modalities.v
@@ -10,9 +10,9 @@ From self.lang Require Import memory.
 From self.high Require Import dprop resources.
 
 Program Definition post_fence {Σ} (P : dProp Σ) : dProp Σ :=
-  MonPred (λ tv, P (store_view tv,
-                    (flush_view tv ⊔ buffer_view tv),
-                    buffer_view tv)) _.
+  MonPred (λ TV, P (store_view TV,
+                    (flush_view TV ⊔ buffer_view TV),
+                    buffer_view TV)) _.
   (* MonPred (λ '(s, p, b), P (s, (p ⊔ b), ∅)) _. *)
 Next Obligation.
   intros Σ P. intros [[??]?] [[??]?] [[??]?]. simpl.
@@ -25,7 +25,7 @@ Qed.
 Notation "'<fence>' P" := (post_fence P) (at level 20, right associativity) : bi_scope.
 
 Program Definition no_buffer `{Σ : gFunctors} (P : dProp Σ) : dProp Σ :=
-  MonPred (λ tv, P (store_view tv, flush_view tv, ∅)) _.
+  MonPred (λ TV, P (store_view TV, flush_view TV, ∅)) _.
 Next Obligation.
   intros Σ P. intros [[??]?] [[??]?] [[??]?]. simpl.
   apply monPred_mono.
@@ -35,3 +35,15 @@ Qed.
 
 Notation "'<nobuf>' P" :=
   (no_buffer P) (at level 20, right associativity) : bi_scope.
+
+Program Definition no_flush `{Σ : gFunctors} (P : dProp Σ) : dProp Σ :=
+  MonPred (λ TV, P (store_view TV, ∅, ∅)) _.
+Next Obligation.
+  intros Σ P. intros [[??]?] [[??]?] [[??]?]. simpl.
+  apply monPred_mono.
+  rewrite !subseteq_prod'.
+  done.
+Qed.
+
+Notation "'<noflush>' P" :=
+  (no_flush P) (at level 20, right associativity) : bi_scope.
